```math
\begin{aligned}
f(x) &= \frac{1}{\sqrt{2\pi\sigma^2}} e^{ -\frac{(x - \mu)^2}{2\sigma^2} } + \int_{-\infty}^{\infty} \left( \sum_{n=1}^{\infty} \frac{(-1)^{n+1} x^n}{n} \right) \cdot \left( \lim_{x \to 0} \frac{\sin x}{x} \right) dx \\
&+ \sum_{n=1}^{\infty} \left( \frac{1}{n^2} - \frac{1}{(n+1)^2} \right) + \prod_{n=1}^{\infty} \left(1 - \frac{x^2}{\pi^2 n^2} \right) \\
&+ \left( \frac{d}{dx} \left[ x^x \right] \right) + \int_0^1 x^{x} dx + \zeta(s) = \frac{1}{\Gamma(s)} \int_0^\infty \frac{x^{s-1}}{e^x - 1} dx
\end{aligned}
```
